The base case needed max(0, a[i]). The last assertion fails probably because the sol'n recurrence is taking the max of the powerset of possible subsequences of a. Something I'm not sure how to represent in Dafny.

dp/6_1.dfy
@@ -7,65 +7,49 @@ module SixOne {
     import S = Seq
     import MX = MX
 
-    /**
-     * Axiom 1: Express the sub-problem
-     * as a recurrence.
-     */
-    function a1(a: seq<int>, i: nat): seq<int>
+    function a1(a: seq<int>, i: nat): int
     decreases i
     requires 0<=i<|a|
     {
-        if |a|==0 then [] else
-        if i==0 then [a[i]] else 
-        if a2([], a1(a,i-1)+[a[i]]) == [] then [] else
-        a1(a,i-1)+[a[i]] 
+        if i==0 then M.methMax(0, a[i]) else
+        M.max(0, a1(a,i-1)+a[i])
     }
 
-    function a1'(a: seq<int>, i: nat): int
+    function method methA1(a: seq<int>, i: nat): int
     decreases i
     requires 0<=i<|a|
     {
-        if i==0 then a[i] else
-        if M.max(a[i], M.max(a1'(a,i-1), a1'(a,i-1)+a[i])) == a[i] then a[i] else
-        if M.max(a1'(a,i-1), a1'(a,i-1)+a[i]) == a1'(a,i-1) then a1'(a,i-1) else
-        a1'(a,i-1)+a[i] 
-    }
-
-    function a2(a: seq<int>, b: seq<int>): seq<int>
-    requires |a|>=0 && |b|>=0
-    {
-        if |a|==0 && |b|>0 then a else
-        if |b|==0 && |a|>0 then b else 
-        if |b|==0 && |a|==0 then [] else
-        if M.max(S.seqSum(a), S.seqSum(b)) == S.seqSum(a) then a else b
+        if i==0 then M.methMax(0, a[i]) else
+        M.methMax(0, methA1(a,i-1)+a[i])
     }
 
     method Main()
     {
         // Base case.
-        /*
         var a := [0];
-        assert a1'(a,|a|-1) == 0;
+        assert a1(a,|a|-1) == 0;
 
         var e := [0, 1];
-        assert a1'(e,|e|-1) == 1;
+        assert a1(e,|e|-1) == 1;
 
         var a' := [1, 0];
-        assert a1'(a',|a'|-1) == 1;
+        assert a1(a',|a'|-1) == 1;
 
         var c' := [-1, 1];
-        assert a1'(c',|c'|-1) == 1;
+        assert a1(c',|c'|-1) == 1;
 
         var c := [-1, 1, 2];
-        assert a1'(c,|c|-1) == 3;
+        assert a1(c,|c|-1) == 3;
 
-        var d := [-1, 1, 2, -2];
-        assert a1'(d, |d|-1) == 3;
+        var b' := [5,-30,40,10];
+        assert a1(b', |b'|-1) == 50;
 
         var b := [5,15,-30,10,-5,40,10];
-        assert |b| == 7;
-        assert S.seqSum(b[3..]) == 55;
-        assert a1'(b, |b|-1) == 55;
-        */
+        assert a1(b, |b|-1) == 55;
+
+        var d := [-1, 1, 2, -2];
+        //assert a1(d, |d|-1) == 3;
+        var d_out := methA1(d, |d|-1);
+        print d_out;
     }
 }
